New decompilation example

examples/l3-machine-code/decompiler/arm_decomp_demoScript.sml
@@ -3,7 +3,7 @@ open HolKernel Parse boolLib bossLib;
 
 val _ = new_theory "arm_decomp_demo";
 
-val (result,func) = arm_decompLib.l3_arm_decompile "PID_C" `
+val (PID_C_cert,PID_C_def) = arm_decompLib.l3_arm_decompile "PID_C" `
             (* ------ PID example ------- *)
   ed907a00  (*  vldr      s14, [r0]       *)
   edd16a00  (*  vldr      s13, [r1]       *)
@@ -23,9 +23,9 @@ val (result,func) = arm_decompLib.l3_arm_decompile "PID_C" `
   ee767aa7  (*  vadd.f32  s15, s13, s15   *)
   edc37a00  (*  vstr      s15, [r3]       *)`;
 
-val _ = save_thm("PID_C_cert",result);
+val _ = save_thm("PID_C_cert",PID_C_cert);
 
-val (result,func) = arm_decompLib.l3_arm_decompile "PID_ADA" `
+val (PID_ADA_cert,PID_ADA_def) = arm_decompLib.l3_arm_decompile "PID_ADA" `
   e3003000  (*  movw      r3, #0          *)
   e3403000  (*  movt      r3, #0          *)
   ed937a00  (*  vldr      s14, [r3]       *)
@@ -43,6 +43,96 @@ val (result,func) = arm_decompLib.l3_arm_decompile "PID_ADA" `
   ee767aa7  (*  vadd.f32  s15, s13, s15   *)
   edc37a06  (*  vstr      s15, [r3, #24]  *)`
 
-val _ = save_thm("PID_ADA_cert",result);
+val _ = save_thm("PID_ADA_cert",PID_ADA_cert);
+
+(* an attempt at proving them equivalent *)
+
+open wordsTheory;
+open wordsLib;
+val _ = (guessing_word_lengths := true);
+
+val word_read_def = Define `
+  word_read (m:word32 -> word8) a =
+    (m (a + 3w) @@ m (a + 2w) @@ m (a + 1w) @@ m (a))`;
+
+val word_write_def = Define `
+  word_write (m:word32 -> word8) (a:word32) (w:word32) =
+           (a + 3w =+ (31 >< 24) w)
+             ((a + 2w =+ (23 >< 16) w)
+                ((a + 1w =+ (15 >< 8) w)
+                   ((a =+ (7 >< 0) w) m)))`;
+
+val put_upper_def = Define `
+  ((put_upper (w:word32) (d:word64)):word64) =
+     bit_field_insert 63 32 w d`;
+
+val put_lower_def = Define `
+  ((put_lower (w:word32) (d:word64)):word64) =
+     bit_field_insert 31 0 w d`;
+
+val get_upper_def = Define `
+  ((get_upper (d:word64)):word32) = (63 >< 32) d`;
+
+val get_lower_def = Define `
+  ((get_lower (d:word64)):word32) = (31 >< 0) d`;
+
+val word_write_lower = prove(
+  ``((a + 3w =+ (31 >< 24) d7)
+     ((a + 2w =+ (23 >< 16) d7)
+      ((a + 1w =+ (15 >< 8) d7)
+       ((a =+ (7 >< 0) d7) m)))) =
+    (word_write m a (get_lower d7))``,
+  SIMP_TAC std_ss [word_write_def,get_lower_def]
+  THEN REPEAT (MATCH_MP_TAC
+   (METIS_PROVE [] ``(x1 = x2) /\ (m1 = m2) ==> ((a =+ x1) m1 = (a =+ x2) m2)``)
+  THEN REPEAT STRIP_TAC THEN SIMP_TAC std_ss [] THEN1 blastLib.BBLAST_TAC));
+
+val word_write_upper = prove(
+  ``((a + 3w =+ (63 >< 56) d7)
+            ((a + 2w =+ (55 >< 48) d7)
+               ((a + 1w =+ (47 >< 40) d7)
+                  ((a =+ (39 >< 32) d7) m)))) =
+    (word_write m a (get_upper d7))``,
+  SIMP_TAC std_ss [word_write_def,get_upper_def]
+  THEN REPEAT (MATCH_MP_TAC
+   (METIS_PROVE [] ``(x1 = x2) /\ (m1 = m2) ==> ((a =+ x1) m1 = (a =+ x2) m2)``)
+  THEN REPEAT STRIP_TAC THEN SIMP_TAC std_ss [] THEN1 blastLib.BBLAST_TAC));
+
+val put_get_simp = prove(
+  ``(put_upper w (put_upper w1 d) = put_upper w d) /\
+    (get_upper (put_upper w d) = w) /\
+    (get_upper (put_lower w1 d) = get_upper d) /\
+    (put_lower w (put_lower w1 d) = put_lower w d) /\
+    (get_lower (put_lower w d) = w) /\
+    (get_lower (put_upper w1 d) = get_lower d) /\
+    (put_upper w1 (put_lower w2 d) = put_lower w2 (put_upper w1 d))``,
+  SIMP_TAC std_ss [put_lower_def,get_lower_def,put_upper_def,get_upper_def]
+  THEN blastLib.BBLAST_TAC);
+
+val lemma = EVAL ``bit_field_insert 31 16 (0w:word16) (0w:word32) : word32``
+
+val PID_ADA_lemma =
+  PID_ADA_def |> CONJUNCT1 |> SIMP_RULE std_ss [GSYM word_read_def,
+    GSYM put_upper_def,GSYM put_lower_def,word_write_lower,word_write_upper,
+    GSYM get_lower_def,GSYM get_upper_def,Once LET_DEF,lemma]
+  |> SIMP_RULE std_ss [LET_DEF,put_get_simp,word_add_n2w]
+
+val PID_C_lemma =
+  PID_C_def |> CONJUNCT1 |> SIMP_RULE std_ss [GSYM word_read_def,
+    GSYM put_upper_def,GSYM put_lower_def,word_write_lower,word_write_upper,
+    GSYM get_lower_def,GSYM get_upper_def,Once LET_DEF,lemma]
+  |> SIMP_RULE std_ss [LET_DEF,put_get_simp,word_add_n2w,lemma]
+
+val PID_ADA_EQUIV_PID_C = store_thm("PID_ADA_EQUIV_PID_C",
+  ``(word_read m2 r0 = word_read m1 0w) /\
+    (word_read m2 0w = word_read m1 4w) /\
+    (word_read m2 r3 = word_read m1 8w) /\
+    (word_read m2 r2 = word_read m1 16w) ==>
+    let (r3_a,d5_a,d6_a,d7_a,dm_a,m_a,rmode_a) =
+            PID_ADA (d5,d6,d7,dm,m1,rmode) in
+    let (r0_c,r1_c,r2_c,r3_c,r13_c,d5_c,d6_c,d7_c,dm_c,m_c,rmode_c) =
+            PID_C (r0,r1,r2,r3,r13,d5,d6,d7,dm,m2,rmode) in
+      (d7_a,rmode_a) = (d7_c,rmode_c)``,
+  SIMP_TAC std_ss [PID_ADA_lemma,PID_C_lemma,LET_DEF]);
 
 val _ = export_theory();
